Last updates

ClassicalFunctional.fst
@@ -1,1 +1,73 @@
 module ClassicalFunctional
+let rec length (#a: Type) (l: list a)
+  : Tot nat (decreases l) = 
+  match l with
+  | [] -> 0
+  | _ :: l' -> 1 + length l'
+
+val append #a (xs ys: list a) 
+  : l: list a {length l = length xs + length ys}
+let rec append xs ys = 
+  match xs with
+  | [] -> ys
+  | x :: xs' -> x :: append xs' ys
+
+let rec append_two_lists (#a: Type) (xs ys: list a)
+  : Lemma (length (append xs ys) == length xs + length ys)
+  = match xs with
+  | [] -> ()
+  | _ :: xs' -> append_two_lists xs' ys
+
+let rec append_associative #a (ls xs ys: list a)
+  : Lemma (ensures append (append ls xs) ys == append ls (append xs ys))
+  = match ls with
+  | [] -> ()
+  | l :: ls' -> append_associative ls' xs ys
+
+let rec reverse (#a: Type) (l:list a)
+  : list a
+  = match l with
+  | [] -> []
+  | hd :: tl -> append (reverse tl) [hd]
+
+let rec foldLeft #a #b (f: b -> a -> a) (ls: list b) (acc:a)
+  : a
+  = match ls with
+  | [] -> acc
+  | l :: ls' -> foldLeft f ls' (f l acc)
+
+let rec sum (xs: list int)
+  : Tot int (decreases xs)
+  = match xs with
+  | [] -> 0
+  | x :: xs' -> x + sum xs'
+
+let rec foldLeft_and_sum_general (acc: int) (xs: list int)
+  : Lemma (ensures foldLeft (+) xs acc == acc + sum xs)
+          (decreases length xs)
+  = match xs with
+  | [] -> ()
+  | x :: xs' -> foldLeft_and_sum_general (x + acc) xs'
+  
+let foldLeft_and_sum (xs: list int)
+  : Lemma (ensures foldLeft (+) xs 0 == sum xs)
+  = foldLeft_and_sum_general 0 xs
+
+let rec append_list_on_empty (#a: Type) (ls: list a)
+  : Lemma (append ls [] == ls)
+  = match ls with
+  | [] -> ()
+  | _ :: ls' -> append_list_on_empty ls'
+
+let rec foldLeft_cons_is_rev_general (#a: Type) (ls xs: list a)
+  : Lemma (ensures foldLeft Cons ls xs == append (reverse ls) xs)
+  = match ls with
+  | [] -> ()
+  | l :: ls' -> 
+    append_associative (reverse ls') [l] xs;
+    foldLeft_cons_is_rev_general ls' (l :: xs)
+
+let foldLeft_Cons_is_rev (#a: Type) (ls: list a)
+  : Lemma (foldLeft Cons ls [] == reverse ls)
+  = append_list_on_empty (reverse ls);
+    foldLeft_cons_is_rev_general ls []
