SimpleInduction.fst
@@ -12,3 +12,37 @@ let rec sum1_value (n: nat)
   = match n with
     | 0 -> ()
     | _ -> sum1_value (n - 1)
+
+let rec fibonacci (n:nat)
+  : nat
+  = if n <= 1 then 1 
+  else fibonacci (n - 1) + fibonacci (n - 2)
+
+let rec g (a b n : nat)
+  : Tot nat (decreases n)
+  = match n with
+  | 0 -> a
+  | _ -> g b (a+b) (n-1)
+
+let rec general_G_relation (a b n: nat)
+  : Lemma (ensures
+      g a b 0 == a /\ 
+      g a b 1 == b /\
+      n >= 2 ==> g a b n == g a b (n - 1) + g a b (n - 2)
+  )
+  (decreases n)
+  = match n with
+  | 0 -> ()
+  | 1 -> ()
+  | _ -> 
+      general_G_relation b (a + b) (n - 1)
+
+let rec g_is_okay (n: nat)
+  : Lemma (ensures g 1 1 n == fibonacci n)
+          (decreases n)
+  = match n with
+  | 0 | 1 -> ()
+  | _ ->
+      general_G_relation 1 1 n;
+      g_is_okay (n - 1);
+      g_is_okay (n - 2)
