NewContextFreeGrammars.fst
@@ -1,0 +1,245 @@
+module NewContextFreeGrammars
+open FStar.List
+open FStar.String
+
+// Implementation 
+type variable_type = 
+  | Var of string
+type terminal_type = 
+  | Term of string
+type variables = list variable_type // (finite) set of variables
+type terminals = list terminal_type // (finite) set of terminals
+type rhs' = 
+  | T of terminal_type
+  | V of variable_type
+type rhs_type = (ls: list rhs'{List.length ls >= 1})
+type production_type = variable_type * rhs_type
+type start = variable_type
+
+type cfg_type = {
+  variables: variables;
+  terminals: terminals;
+  productions: list production_type;
+  start: start
+}
+
+type derivation_state = list rhs' * option variable_type * list rhs'
+
+let cfg_a: cfg_type = {
+  variables = [Var "A"];
+  terminals = [Term "a"];
+  productions = [
+    (Var "A", [T (Term "a")]);
+    (Var "A", [V (Var "A"); T (Term "a")])
+  ];
+  start = Var "A"
+}
+
+let move_everything_right (state: derivation_state) 
+  : derivation_state
+  = match state with 
+    | (left, None, right) -> ([], None, List.append left right)
+    | (left, Some var, right) -> ([], None, List.append left ((V var) :: right))
+
+let is_middle_none (state: derivation_state)
+  : bool 
+  = match state with 
+    | (_, None, _) -> true 
+    | _ -> false
+
+let get_right (state: derivation_state)
+  : list rhs' 
+  = match state with 
+    | (_, _, right) -> right
+
+let get_left (state: derivation_state)
+  : list rhs' 
+  = match state with 
+    | (left, _, _) -> left
+
+let rec all_variable_states (state: derivation_state{is_middle_none state}) (var: variable_type)
+  : Tot (list derivation_state) (decreases get_right state)
+  = match state with 
+    | (left, None, []) -> []
+    | (left, None, T t :: right') -> 
+      all_variable_states (List.append left [T t], None, right') var
+    | (left, None, V var' :: right') -> 
+      if var' = var then (left, Some var, right') :: all_variable_states (List.append left [V var], None, right') var
+      else all_variable_states (List.append left [V var'], None, right') var
+
+let rec count_variable (ls: list rhs') (var: variable_type)
+  : nat 
+  = match ls with 
+    | [] -> 0 
+    | T _ :: ls' -> count_variable ls' var
+    | V var' :: ls' -> count_variable ls' var + (if var' = var then 1 else 0)
+
+let count_variable_state (state: derivation_state) (var: variable_type)
+  : nat 
+  = match state with 
+    | (left, None, right) -> count_variable left var + count_variable right var
+    | (left, Some var, right) -> 1 + count_variable left var + count_variable right var
+
+let apply_production_rule (state: derivation_state) (production: production_type)
+  : option derivation_state
+  = let (var, rhs) = production in 
+    match state with 
+    | (left, None, right) -> None
+    | (left, Some var', right) -> 
+        if var' = var then Some (left, None, List.append rhs right)
+        else None
+
+let rec derivation_step (states: list derivation_state) (production: production_type)
+  : Tot (list derivation_state) (decreases states)
+  = match states with 
+    | [] -> []
+    | state :: states' -> 
+      begin
+        match apply_production_rule state production with 
+        | None -> derivation_step states' production
+        | Some state' -> state' :: derivation_step states' production
+      end
+
+let rec power_step (state: derivation_state) (productions: list production_type)
+  : Tot (list derivation_state) (decreases productions)
+  = match productions with
+    | [] -> []
+    | (var, rhs) :: productions' -> 
+        let state_right = move_everything_right state in 
+        let states = all_variable_states state_right var in
+        List.append (derivation_step states (var, rhs)) (power_step state productions')
+
+let rec power_step_list (states: list derivation_state) (productions: list production_type)
+  : Tot (list derivation_state) (decreases states)
+  = match states with 
+    | [] -> []
+    | state :: states' ->
+      List.append (power_step state productions) (power_step_list states' productions)
+
+let rec n_power_steps (states: list derivation_state) (productions: list production_type) (n: pos)
+  : Tot (list derivation_state) (decreases n)
+  = match n with 
+    | 1 -> power_step_list states productions
+    | _ -> n_power_steps (power_step_list states productions) productions (n - 1)
+
+let n_power_steps_test_lemma _ 
+  : Lemma (ensures 
+            n_power_steps [([], Some (Var "A"), [])] cfg_a.productions 3 == [
+                                                                              ([], None, [T (Term "a"); T (Term "a"); T (Term "a")]);
+                                                                              ([], None, [V (Var "A"); T (Term "a"); T (Term "a"); T (Term "a")])
+                                                                            ]
+          )
+  = normalize_term_spec (n_power_steps [([], Some (Var "A"), [])] cfg_a.productions 3)
+
+let rec only_terminals (xs: list rhs')
+  : bool 
+  = match xs with 
+    | [] -> true
+    | T _ :: xs' -> only_terminals xs' 
+    | V _ :: xs' -> false 
+
+let is_word (state: derivation_state)
+  : bool 
+  = match state with 
+    | (left, None, right) -> only_terminals left && only_terminals right
+    | _ -> false
+
+let word_in_language (word: derivation_state{is_word word}) (cfg: cfg_type) (n: pos)
+  : bool 
+  = List.contains word (n_power_steps [([], Some cfg.start, [])] cfg.productions n)
+
+let word_in_language_test_lemma _ 
+  : Lemma (ensures word_in_language ([], None, [T (Term "a"); T (Term "a"); T (Term "a")]) cfg_a 3)
+  = normalize_term_spec (word_in_language ([], None, [T (Term "a"); T (Term "a"); T (Term "a")]) cfg_a 3)
+
+// Transformation
+let rec handle_rhs (rhs: rhs_type) (terminal_to_replace: terminal_type) (new_variable: variable_type)
+  : (ls: rhs_type{List.length ls >= 1})
+  = match rhs with
+    | [T t] -> 
+      if t = terminal_to_replace then [V new_variable]
+      else [T t]
+    | [V v] -> [V v]
+    | T t :: rhs' -> 
+      if t = terminal_to_replace then 
+        V new_variable :: handle_rhs rhs' terminal_to_replace new_variable
+      else 
+        T t :: handle_rhs rhs' terminal_to_replace new_variable
+    | V v :: rhs' -> 
+      V v :: handle_rhs rhs' terminal_to_replace new_variable
+
+let rec handle_productions (productions: list production_type) (terminal_to_replace: terminal_type) (new_variable: variable_type)
+  : list production_type
+  = match productions with 
+    | [] -> []
+    | (var, rhs) :: productions' -> 
+      let new_rhs = handle_rhs rhs terminal_to_replace new_variable in 
+      (var, new_rhs) :: handle_productions productions' terminal_to_replace new_variable
+
+let handle_productions_test_lemma _ 
+  : Lemma (ensures handle_productions cfg_a.productions (Term "a") (Var "C0") == [(Var "A", [V (Var "C0")]);
+                                                                                  (Var "A", [V (Var "A"); V (Var "C0")])
+                                                                                ]
+          )
+  = normalize_term_spec (handle_productions cfg_a.productions (Term "a") (Var "C0"))
+
+let valid_substitution (cfg: cfg_type) (terminal_to_replace: terminal_type) (new_variable: variable_type)
+  : bool 
+  = List.contains terminal_to_replace cfg.terminals && 
+    not (List.contains new_variable cfg.variables)
+
+let remove_terminal_and_introduce_variable (cfg: cfg_type) (terminal_to_replace: terminal_type) (new_variable: variable_type)
+  : cfg_type
+  = let updated_productions = handle_productions cfg.productions terminal_to_replace new_variable in 
+    { cfg with
+        productions = (new_variable, [T terminal_to_replace]) :: updated_productions; 
+        variables = new_variable :: cfg.variables }
+
+let remove_terminal_and_introduce_variable_test_lemma _ 
+  : Lemma (ensures 
+            remove_terminal_and_introduce_variable cfg_a (Term "a") (Var "C0") == { 
+                                                                                    variables = [Var "C0"; Var "A"];
+                                                                                    terminals = [Term "a"];
+                                                                                    productions = [
+                                                                                      (Var "C0", [T (Term "a")]);
+                                                                                      (Var "A", [V (Var "C0")]);
+                                                                                      (Var "A", [V (Var "A"); V (Var "C0")]);
+                                                                                    ];
+                                                                                    start = Var "A"
+                                                                                  }
+          )
+  = normalize_term_spec (remove_terminal_and_introduce_variable cfg_a (Term "a") (Var "C0"))
+
+// Properties
+let one_more_variable (cfg: cfg_type) (terminal_to_replace: terminal_type) (new_variable: variable_type)
+  : Lemma (requires valid_substitution cfg terminal_to_replace new_variable)
+          (ensures 
+            List.length cfg.variables + 1 == 
+            List.length (remove_terminal_and_introduce_variable cfg terminal_to_replace new_variable).variables
+          )
+  = ()
+
+let simplify_word (state: derivation_state)
+  : derivation_state
+  = match state with 
+    | (left, None, right) -> ([], None, List.append left right)
+    | (left, Some var, right) -> ([], None, List.append left ((V var) :: right))
+
+let original_is_in_new_general (word: derivation_state{is_word word}) (state: derivation_state) (cfg cfg': cfg_type) (terminal_to_replace: terminal_type) (new_variable: variable_type)
+  : Lemma (requires 
+            valid_substitution cfg terminal_to_replace new_variable /\
+            cfg' == remove_terminal_and_introduce_variable cfg terminal_to_replace new_variable /\
+            exists (n: pos). word_in_language word cfg n
+          )
+          (ensures 
+            exists (n': pos). word_in_language word cfg' n'
+          )
+  = ()
+
+let rec all_variable_states_length (state: derivation_state) (var: variable_type)
+  : Lemma (ensures 
+            List.length (all_variable_states (move_everything_right state) var)
+            == count_variable_state state var
+          )
+  = match move_everything_right state with 
+    | ([], None, right) -> ()
