old_context_free_grammars/ContextFreeGrammarsProperties.fst
@@ -1,0 +1,150 @@
+module ContextFreeGrammarsProperties
+open FStar.List
+open FStar.String
+open ContextFreeGrammars
+
+type yep = 
+  | POS of int
+  | NEG of int
+
+let rec remove_negative (xs: list yep)
+  : Tot (list yep) (decreases xs)
+  = match xs with
+    | [] -> []
+    | POS x :: xs' -> POS x :: remove_negative xs'
+    | NEG x :: xs' -> remove_negative xs' 
+
+let rec is_positive (xs: list yep)
+  : Tot (bool) (decreases xs)
+  = match xs with
+    | [] -> true
+    | POS _ :: xs' -> is_positive xs'
+    | NEG _ :: _ -> false
+
+let rec t (xs: list yep)
+  : Lemma (ensures is_positive (remove_negative xs))
+  = match xs with
+    | [] -> ()
+    | _ :: xs' -> t xs'
+
+// Properties
+let no_eps_symbol (cfg: cfg_type)
+  : bool 
+  = not (List.contains (Term "") cfg.terminals) &&
+    for_all (
+      fun (_, rhs) -> 
+        not (List.contains (T (Term "")) rhs)
+    ) cfg.productions
+
+let rec check (rhs: rhs_type)
+  : Tot (bool) (decreases rhs)
+  = match rhs with
+    | [] -> true
+    | V _ :: rhs' -> true && check rhs'
+    | T _ :: rhs' -> false 
+
+let rec no_unit_productions' (productions: list production_type)
+  : bool
+  = match productions with
+    | [] -> true
+    | [_, [V _]] -> false
+    | _ :: productions' -> no_unit_productions' productions'
+
+let no_unit_productions (cfg: cfg_type)
+  : bool 
+  = no_unit_productions' cfg.productions
+
+// Construction for a
+let rec convert_AST_a_to_AST (ast_a: ast_type) (cfg: cfg_type)
+  : list ast_type
+  = match ast_a with
+    | Node (var, [T' t]) -> 
+      if List.contains var cfg.variables then 
+        [ast_a]
+      else 
+        [T' t]
+    | Node (var, ast_a_list) -> 
+        [Node (var, convert_AST_a_to_AST_list ast_a_list cfg)]
+    | T' t -> [T' t]
+and convert_AST_a_to_AST_list (ast_a_list: list ast_type) (cfg: cfg_type)
+  : list ast_type
+  = match ast_a_list with 
+    | [] -> [] 
+    | ast :: ast_a_list' -> 
+      List.append (convert_AST_a_to_AST ast cfg) (convert_AST_a_to_AST_list ast_a_list' cfg)
+
+let a_CF_construction_a = {
+  variables = [Var "A"; Var "Z0"];
+  terminals = [Term "a"; Term "+"];
+  productions = [
+    (Var "A", [T (Term "a")]);
+    (Var "A", [V (Var "A"); V (Var "Z0"); V (Var "A")]);
+    (Var "Z0", [T (Term "+")])
+  ];
+  start = Var "A"
+}
+let aPaPa_construction_a = 
+  Node (Var "A", [
+    Node (Var "A", [T' (Term "a")]);
+    Node (Var "Z0", [T' (Term "+")]);
+    Node (Var "A", [
+      Node (Var "A", [T' (Term "a")]);
+      Node (Var "Z0", [T' (Term "+")]);
+      Node (Var "A", [T' (Term "a")])
+    ])
+  ])
+
+let ttt _ 
+  : Lemma (convert_AST_a_to_AST aPaPa_construction_a a_CFG == [aPaPa])
+  = normalize_term_spec (convert_AST_a_to_AST aPaPa_construction_a a_CFG)
+
+let rec ast_to_list (ast: ast_type) 
+  : list terminal_type 
+  = match ast with 
+    | Node (var, ast_list) -> 
+      ast_to_list_list ast_list
+    | T' t -> [t]
+and ast_to_list_list (ast_list: list ast_type)
+  : list terminal_type
+  = match ast_list with 
+    | [] -> []
+    | ast :: ast_list' -> 
+      List.append (ast_to_list ast) (ast_to_list_list ast_list')
+
+let tttt _ 
+  : Lemma (
+            ast_to_list aPaPa == [Term "a"; Term "+"; Term "a"; Term "+"; Term "a"] /\
+            ast_to_list aPaPa_CNF == [Term "a"; Term "+"; Term "a"; Term "+"; Term "a"]
+          )
+  = normalize_term_spec (ast_to_list aPaPa);
+    normalize_term_spec (ast_to_list aPaPa_CNF)
+
+let rec construction_a_lemma_1 (ast ast_a: ast_type) (cfg cfg_a: cfg_type)
+  : Lemma (requires 
+            cfg_a == construction_a cfg /\
+            ast_in_cfg ast_a cfg_a /\
+            [ast] == convert_AST_a_to_AST ast_a cfg
+          )
+          (ensures ast_to_list ast_a == ast_to_list ast)
+  = match ast with 
+
+let construction_a_lemma_2 (ast ast_a: ast_type) (cfg cfg_a: cfg_type)
+  : Lemma (requires 
+            cfg_a == construction_a cfg /\
+            ast_in_cfg ast_a cfg_a /\
+            [ast] == convert_AST_a_to_AST ast_a cfg
+          )
+          (ensures ast_in_cfg ast cfg)
+  = ()
+
+// End goal
+// let rec cnf_in_original (ast ast_CNF: ast_type) (cfg cfg_CNF: cfg_type)
+//   : Lemma (requires 
+//             cfg_CNF == entire_construction cfg /\
+//             ast_in_cfg ast_CNF cfg_CNF
+//           )
+//           (ensures 
+//             ast == (Cons?.hd (convert_AST_CNF_to_AST ast_CNF cfg)) /\
+//             ast_in_cfg ast cfg
+//           )
+//   = () 
